src/Iris/Std/PartialMap.lean
@@ -90,6 +90,20 @@ class LawfulPartialMap (M : Type _ → Type _) (K : outParam (Type _)) [PartialM
   get?_delete_ne {m : M V} {k k'} : k ≠ k' → get? (delete m k) k' = get? m k'
 export LawfulPartialMap (get?_empty get?_insert_eq get?_insert_ne get?_delete_eq get?_delete_ne)
 
+/-- A functorial partial map is a partial map, whose functor map function preserves the non-allocation
+    of elements. -/
+class FunctorialPartialMap (M : Type _ → Type _) (K : outParam (Type _))
+    extends PartialMap M K, Functor M where
+  get?_map {m : M V} {f : K → V → Option V'} {k} :
+    get? (f k <$> m) k = (get? m k).bind (f k)
+export FunctorialPartialMap (get?_map)
+
+theorem map_some [FunctorialPartialMap M K] {m : M V} {f : K → V → Option V'} (H : get? m k = some v) :
+    get? (f k <$> m) k = f k v := by simp [get?_map, H]
+
+theorem map_none [FunctorialPartialMap M K] {m : M V} {f : K → V → Option V'} (H : get? m k = none) :
+    get? (f k <$> m) k = none := by simp [get?_map, H]
+
 namespace PartialMap
 
 variable {K : Type v} {M : Type u → _} [PartialMap M K]
